01_Introduction.thy
@@ -1,7 +1,6 @@
 (*<*)
 theory "01_Introduction"
   imports
-    "../Examples"
     "HOL-Library.LaTeXsugar"
 begin
 (*>*)
@@ -12,7 +11,6 @@ text\<open>
   \begin{itemize}
     \item How much explain the proofs? \\
     \item How reference thm names? \\
-    \item How to get rid of where? \\
     \item How to tum blau assumes shows fun ... keywords? \\
   \end{itemize}
 \<close>
@@ -24,6 +22,53 @@ section\<open>Earley\<close>
 section\<open>Jones\<close>
 
 section\<open>Scott\<close>
+
+section\<open>Aycock\<close>
+
+section\<open>Related Work\<close>
+
+subsection\<open>Related Parsing Algorithms\<close>
+
+text\<open>Tomita \cite{Tomita:1987} presents an generalized LR parsing algorithm for augmented
+context-free grammars that can handle arbitrary context-free grammars.
+
+Izmaylova \textit{et al} \cite{Izmaylova:2016} develop a general parser 
+combinator library based on memoized Continuation-Passing Style (CPS) recognizers that supports all
+context-free grammars and constructs a Shared Packed Parse Forest (SPPF) in worst case cubic time and space.
+\<close>
+
+subsection\<open>Related Verification Work\<close>
+
+text\<open>TODO: LocalLexing!!!\<close>
+
+text\<open>
+Obua \textit{et al} \cite{Obua:2017} introduce local lexing, a novel parsing concept which interleaves
+lexing and parsing whilst allowing lexing to be dependent on the parsing process. They base their
+development on Earley's algorithm and have verified the correctness with respect to its local lexing
+semantics in the theorem prover Isabelle/HOL. The background theory of this Master's thesis is based
+upon the local lexing entry \cite{LocalLexing-AFP} in the Archive of Formal Proofs.
+
+Lasser \textit{et al} \cite{Lasser:2019} verify an LL(1) parser generator using the Coq proof assistant.
+
+Barthwal \textit{et al} \cite{Barthwal:2009} formalize background theory
+about context-free languages and grammars, and subsequently verify an SLR automaton and parser produced
+by a parser generator.
+
+Blaudeau \textit{et al} \cite{Blaudeau:2020} formalize the metatheory on Parsing expression grammars (PEGs) and
+build a verified parser interpreter based on higher-order parsing combinators for expression grammars
+using the PVS specification language and verification system. Koprowski \textit{et al} \cite{Koprowski:2011}
+present TRX: a parser interpreter formally developed in Coq which also parses expression grammars.
+
+Jourdan \textit{et al} \cite{Jourdan:2012} present a validator which checks if a context-free grammar
+and an LR(1) parser agree, producing correctness guarantees required by verified compilers.
+
+Lasser \textit{et al} \cite{Lasser:2021} present the verified parser CoStar based on the ALL(*) algorithm.
+They proof soundness and completeness for all non-left-recursive grammars using the Coq proof assistant.
+
+
+\<close>
+
+section\<open>Future Work\<close>
 
 chapter\<open>Introduction\<close>
 
@@ -45,11 +90,6 @@ text\<open>see folder and bibliography\<close>
 section\<open>Contributions\<close>
 
 text\<open>what did I do, what is new\<close>
-
-section \<open>Isabelle/HOL\<close>
-
-text\<open>take closest pair paper section and add additional notation as needed, also discuss
-the different representations of lemmas and definitions (separate or within the text)\<close>
 
 (*<*)
 end
